Upgrade to Dafny 2.0.0
Update function types to the new long arrow syntax: regular arrows
("->") not seem to stand for total functions, not the partial functions
that they used to denote.  The new syntax for partial functions is
through either "-->" for functions that may not read from the heap and
"~>" for those that may. We go for "-->" as a first step; yet in the
future we may want to benefit from Dafny's total functions, following
the Dijkstra and Scholten assumption(from their 1990 Monograph
"Predicate Calculus and Program Semantics").

Having modified all functions to "-->", all "reads" clauses were
removed. (They were anyway redundant: the vast majority of these clauses
were the unhelpful "reads *", that had been introduced merely to silence
Dafny's concerns.)

In addition, "this" can no longer be referred to in a precondition to a
constructor - so for now the postcondition of the VariablesSSA
constructor is commented out, as it is otherwise not guaranteed to hold,
since the forced removal of the (proably incorrect)  precondition that
it held on entry to the constructor.

Definitions.dfy
@@ -7,17 +7,17 @@ datatype Statement = Assignment(LHS: seq<Variable>, RHS: seq<Expression>) | Skip
 		LocalDeclaration(L: seq<Variable>, S0: Statement) | Live(L: seq<Variable>, S0: Statement) | Assert(B: BooleanExpression)
 type Variable = string
 datatype Value = Int(i: int) | Bool(b: bool)
-type Expression = (State -> Value, set<Variable>)
-type BooleanExpression = (State -> bool, set<Variable>) 
+type Expression = (State --> Value, set<Variable>)
+type BooleanExpression = (State --> bool, set<Variable>) 
 type State = map<Variable, Value>
-type Predicate = (State -> bool, set<Variable>)
+type Predicate = (State --> bool, set<Variable>)
 
 
 //============================================================
 //					*** Validation ***
 //============================================================
 
-predicate Valid(stmt: Statement) reads *
+predicate Valid(stmt: Statement)
 {
 	match stmt {
 		case Skip => true
@@ -120,7 +120,7 @@ function method ExpressionListToString(expressions: seq<Expression>) : string
 function EqualityAssertion(X: seq<Variable>, E: seq<Expression>): (assertion: Statement)
 	requires ValidAssignment(X,E)
 {
-	var B := ((state: State) reads * 
+	var B := ((state: State)
 		requires (forall i :: 0 <= i < |X| ==> X[i] in state && E[i].0.requires(state)) => 
 		forall i :: 0 <= i < |X| ==> state[X[i]] == E[i].0(state), 
 		setOf(X)+varsInExps(E));
@@ -142,30 +142,27 @@ function ConstantPredicate(b: bool): Predicate
 //					*** Definitions ***
 //============================================================
 
-function power<T>(f: T->T, i: nat): T->T
+function power<T>(f: T-->T, i: nat): T-->T
 	decreases i
 {
 	if i == 0 then x => x
 	else x
 		requires power(f, i-1).requires(x)
 		requires f.requires(power(f, i-1)(x))
-		reads *
 		=> f(power(f, i-1)(x))
 }
 
-function existsK(i: nat, k: Predicate -> Predicate, state: State): bool
-	reads *
+function existsK(i: nat, k: Predicate --> Predicate, state: State): bool
 	requires forall i: nat :: power.requires(k, i)
 	requires forall i: nat, P: Predicate :: power(k, i).requires(P)
 	requires forall state1: State, P: Predicate  :: P.0.requires(state1)
 {
-	var P := ((_ => false),(set v | v in state));
+	var P: Predicate := ((_ => false),(set v | v in state));
 	exists i: nat :: power(k, i)(P).0(state)
 }
 
 // program,post-condition => wp
 function wp(stmt: Statement, P: Predicate): Predicate
-	reads Valid.reads(stmt)
 	requires Valid(stmt)
 	//requires stmt.LocalDeclaration? ==> vars(P) !! setOf(L)
 {
@@ -174,7 +171,6 @@ function wp(stmt: Statement, P: Predicate): Predicate
 		case Assignment(LHS,RHS) => sub(P, LHS, RHS)
 		case SeqComp(S1,S2) => wp(S1, wp(S2, P))
 		case IF(B0,Sthen,Selse) => var f:= (state: State)
-			reads *
 			requires B0.0.requires(state)
 			requires Valid(Sthen) && wp(Sthen, P).0.requires(state)
 			requires Valid(Selse) && wp(Selse, P).0.requires(state)
@@ -182,13 +178,11 @@ function wp(stmt: Statement, P: Predicate): Predicate
 			(B0.0(state) ==> wp(Sthen, P).0(state)) && (!B0.0(state) ==> wp(Selse, P).0(state));
 			(f,vars(P)-ddef(stmt)+input(stmt))
 		case DO(B,Sloop) => var f:= (state: State)
-			reads * //B.reads
 			requires forall state1: State, P: Predicate  :: P.0.requires(state1)
 			=>
-				(var k: Predicate -> Predicate := Q
+				(var k: Predicate --> Predicate := Q
 				=>
 				var g := ((state: State)
-						reads *
 						requires Valid(Sloop)
 						requires B.0.requires(state) /*&& B.0(state).Bool?*/
 						requires wp(Sloop, Q).0.requires(state)
@@ -202,7 +196,6 @@ function wp(stmt: Statement, P: Predicate): Predicate
 		case LocalDeclaration(L,S0) => wp(S0,P)
 		case Live(L,S0) => wp(S0,P)
 		case Assert(B) => var f:= (state: State)
-			reads *
 			requires B.0.requires(state)
 			requires P.0.requires(state)
 			=> /*B.0(state).Bool? && */
@@ -212,7 +205,6 @@ function wp(stmt: Statement, P: Predicate): Predicate
 }
 
 function wlp(stmt: Statement, P: Predicate): Predicate
-	reads Valid.reads(stmt)
 	requires Valid(stmt)
 	//requires stmt.LocalDeclaration? ==> vars(P) !! setOf(L)
 {
@@ -229,7 +221,6 @@ function sub(P: Predicate, X: seq<Variable>, E: seq<Expression>): Predicate
 	requires |X| == |E|
 {
 	var f:= (state: State)
-	reads *
 	requires StateUpdate.requires(state, X, E, state)
 	requires P.0.requires(StateUpdate(state, X, E, state))
 	=>
@@ -241,7 +232,6 @@ function sub(P: Predicate, X: seq<Variable>, E: seq<Expression>): Predicate
 function StateUpdate(oldState: State, X: seq<Variable>, E: seq<Expression>, newState: State): State
 	requires |X| == |E|
 	requires forall i: nat :: i < |E| ==> E[i].0.requires(oldState)
-	reads *
 {
 	if |X| == 0 then newState else
 	StateUpdate(oldState, X[1..], E[1..], newState[X[0] := E[0].0(oldState)])
@@ -340,8 +330,9 @@ function method {:verify true}seqVarToSeqExpr(seqvars: seq<Variable>): (res:seq<
 	ensures varsInExps(res) == setOf(seqvars)
 {
 	if seqvars == [] then []
-	else 
-		([((s:State)requires(seqvars[0] in s)=>s[seqvars[0]], {seqvars[0]})] + seqVarToSeqExpr(seqvars[1..]))
+	else var f := (s:State)requires(seqvars[0] in s)=>s[seqvars[0]];
+		var exp: Expression := (f, {seqvars[0]});
+		([exp] + seqVarToSeqExpr(seqvars[1..]))
 	
 }
 
@@ -355,7 +346,7 @@ else
 	
 } 
 
-predicate EquivalentPredicates(P1: Predicate, P2: Predicate) reads *
+predicate EquivalentPredicates(P1: Predicate, P2: Predicate)
 {
 	forall s: State :: P1.0.requires(s) && P2.0.requires(s) ==> P1.0(s) == P2.0(s)  
 }
@@ -363,7 +354,7 @@ predicate EquivalentPredicates(P1: Predicate, P2: Predicate) reads *
 lemma EquivalentPredicatesLemma(P1: Predicate, P2: Predicate)
 ensures EquivalentPredicates(P1,P2) <==> (forall s: State :: P1.0.requires(s) && P2.0.requires(s) ==> P1.0(s) == P2.0(s))
 
-predicate EquivalentBooleanExpressions(B1: BooleanExpression, B2: BooleanExpression) reads *
+predicate EquivalentBooleanExpressions(B1: BooleanExpression, B2: BooleanExpression)
 {
 	B1.1 == B2.1 &&
 	(forall s :: B1.0.requires(s) <==> B2.0.requires(s)) &&
@@ -371,7 +362,6 @@ predicate EquivalentBooleanExpressions(B1: BooleanExpression, B2: BooleanExpress
 }
 
 predicate EquivalentStatments(S1: Statement, S2: Statement)
-	reads *
 	requires Valid(S1)
 	requires Valid(S2)
 {
@@ -384,7 +374,6 @@ requires Valid(S2)
 ensures EquivalentStatments(S1, S2) <==> (forall P: Predicate :: EquivalentPredicates(wp(S1,P), wp(S2,P)))
 
 predicate Refinement(S1: Statement, S2: Statement)
-	reads *
 	requires Valid(S1)
 	requires Valid(S2)
 {
@@ -397,7 +386,6 @@ requires Valid(S2)
 ensures Refinement(S1, S2) <==> (forall P: Predicate,s: State :: (wp(S1,P).0(s) ==> wp(S2,P).0(s)))
 
 predicate SliceRefinement(S1: Statement, S2: Statement,V: set<Variable>)
-	reads *
 	requires Valid(S1)
 	requires Valid(S2)
 {
@@ -410,7 +398,6 @@ requires Valid(S2)
 ensures SliceRefinement(S1, S2, V) <==> (forall P: Predicate,s: State :: (vars(P) <= V) ==> ((wp(S1,P).0(s) ==> wp(S2,P).0(s))))
 
 predicate CoSliceRefinement(S1: Statement, S2: Statement,V: set<Variable>)
-	reads *
 	requires Valid(S1)
 	requires Valid(S2)
 {
@@ -434,27 +421,27 @@ function VarsOfPredicateSet(W: set<Predicate>): set<Variable>
 
 function PointwisePredicate(s: State, v: Variable) : Predicate
 {
-	(((s1: State) reads*  => v in s1 && v in s && s[v] == s1[v] ,{v}))
+	(((s1: State) => v in s1 && v in s && s[v] == s1[v] ,{v}))
 }
 
 function AND(P1: Predicate,P2: Predicate): Predicate
 {
-	((s: State) reads * requires P1.0.requires(s) && P2.0.requires(s) => P1.0(s) && P2.0(s),P1.1 + P2.1)
+	((s: State) requires P1.0.requires(s) && P2.0.requires(s) => P1.0(s) && P2.0(s),P1.1 + P2.1)
 }
 
 function OR(P1: Predicate,P2: Predicate): Predicate
 {
-	((s: State) reads * requires P1.0.requires(s) && P2.0.requires(s) => P1.0(s) || P2.0(s),P1.1 + P2.1)
+	((s: State) requires P1.0.requires(s) && P2.0.requires(s) => P1.0(s) || P2.0(s),P1.1 + P2.1)
 }
 
 function IMPLIES(P1: Predicate,P2: Predicate): Predicate  
 {
-	((s: State) reads * requires P1.0.requires(s) && P2.0.requires(s) => P1.0(s) ==> P2.0(s), P1.1 + P2.1) 
+	((s: State) requires P1.0.requires(s) && P2.0.requires(s) => P1.0(s) ==> P2.0(s), P1.1 + P2.1) 
 }
 
 function NOT(P1: Predicate): Predicate  
 {
-	((s: State) reads * requires P1.0.requires(s) => !P1.0(s), P1.1)
+	((s: State) requires P1.0.requires(s) => !P1.0(s), P1.1)
 }
 
 //============================================================
@@ -469,17 +456,17 @@ lemma IdentityOfAND(S: Statement,P1: Predicate)
 requires Valid(S)
 ensures EquivalentPredicates(wp(S,AND(P1,ConstantPredicate(true))),wp(S,P1))
 
-lemma Leibniz<T>(f: Predicate->T, P1: Predicate, P2: Predicate)
+lemma Leibniz<T>(f: Predicate-->T, P1: Predicate, P2: Predicate)
 requires EquivalentPredicates(P1,P2)
 requires f.requires(P1) && f.requires(P2)
 ensures f(P1) == f(P2)
 
-lemma Leibniz2<S,T>(f: (S,Predicate)->T, P1: Predicate, P2: Predicate, s: S)
+lemma Leibniz2<S,T>(f: (S,Predicate)-->T, P1: Predicate, P2: Predicate, s: S)
 requires EquivalentPredicates(P1,P2)
 requires f.requires(s,P1) && f.requires(s,P2)
 ensures f(s,P1) == f(s,P2)
 
-lemma Leibniz3<T>(f: (Statement,Predicate)->T, S: Statement,SV: Statement ,p: Predicate)
+lemma Leibniz3<T>(f: (Statement,Predicate)-->T, S: Statement,SV: Statement ,p: Predicate)
 requires f.requires(S,p) && f.requires(SV,p)
 ensures f(S,p) == f(SV,p)
 
